\documentclass[a4paper,11pt,onecolumn]{scrartcl}

\usepackage[a4paper,left=1.5cm,right=1.5cm,top=1.5cm]{geometry}

\usepackage[utf8]{inputenc} % input encoding        
\usepackage[T1]{fontenc} % font encoding    
\usepackage{lmodern}  		    
\usepackage[english]{babel} % language	              


\usepackage{float} 
\usepackage{graphicx} 
\graphicspath{{Figures/}}                

		
% mathematics                         
\usepackage{amsmath,amsfonts}		
\usepackage{upgreek}
\renewcommand{\vec}{\boldsymbol}
\renewcommand{\i}{\mathrm i}
\newcommand{\e}{\mathrm e}

\usepackage{paralist}

\setlength\fboxsep{0.25cm}
\setlength\fboxrule{0.4pt}

\begin{document}

Given the electromagnetic field $E(x, y, 0)$ defined in the plane $z = 0$, the field $E(x,y,z)$ in the plane $z$ can be calculated using the Fresnel diffraction integral:
\begin{align}
E(x,y,z) = \frac{\mathrm e^{\i kz}}{\i\lambda z}\iint\limits_{-\infty}^{+\infty} E(x', y', 0)\,\e^{\i\frac{k}{2z}\left((x-x')^2 + (y-y')^2\right)\;}\mathrm dx'\mathrm dy'
\end{align}

\begin{align}
E(x,y,z) = E(x, y, 0) 
* h(x,y,z)\ ,
\end{align}
where
\begin{align}
h(x, y, z) = \frac{\mathrm e^{\i kz}}{\i\lambda z}\e^{\i\frac{k}{2z}(x^2 + y^2)}
\end{align}
\begin{align}
(f * g)(x) = \int f(x)\,g(x - x')\,\mathrm dx' 
\end{align}

Since ${\mathcal {F}}\{f*g\}={\mathcal {F}}\{f\}\cdot {\mathcal {F}}\{g\}$
\begin{align}
\check{E}(f_x, f_y, z) = \check{E}(f_x, f_y, 0)H(f_x, f_y, z)
\end{align}

\begin{align}
H(f_x, f_y, z) &= \mathcal F\{h(x, y,z)\} \\
&= \frac{\mathrm e^{\i kz}}{\i\lambda z} \mathcal F\left\{\e^{\i\frac{k}{2z}x^2 }\right\}\mathcal F\left\{\e^{\i\frac{k}{2z}y^2 }\right\}
\end{align}

\begin{align}
\mathcal F\left\{\e^{\i\alpha t^2 }\right\} = \sqrt{\frac{\pi}{\alpha}} \,\e^{\i\frac{\pi}{4}}\,\e^{-\i\frac{(2\pi f)^2}{4\alpha}}
\end{align}

\begin{align}
H(f_x, f_y, z) &= \frac{\mathrm e^{\i kz}}{\i\lambda z}\sqrt{\frac{2\pi z}{k}} \,\e^{\i\frac{\pi}{4}}\,\e^{-\i\frac{4\pi^2 f_x^2 2z}{4k}} \sqrt{\frac{2\pi z}{k}} \,\e^{\i\frac{\pi}{4}}\,\e^{-\i\frac{4\pi^2 f_y^2 2z}{4k}} \\
&=  \frac{\mathrm e^{\i kz}}{\i\lambda z}\frac{2\pi z}{k}\,\e^{-\i\pi\lambda z f_x^2}\,\e^{-\i\pi\lambda z f_y^2} = \e^{\i kz}\e^{-\i\pi\lambda z(f_x^2 + f_y^2)}
\end{align}

\begin{align}
H(f_x, f_y, z) = \e^{\i kz}\e^{-\i\pi\lambda z(f_x^2+f_y^2)}
\end{align}

\begin{align}
\check{E}(f_x, f_y, z) = \e^{\i kz}\e^{-\i\pi\lambda z(f_x^2+f_y^2)}\,\check{E}(f_x, f_y, 0)
\end{align}

Propagate from the SLM plane $E_\mathrm{SLM}(x, y)$ to the lense:
\begin{align}
E_\mathrm{Lense}^-(x,y) = \frac{\mathrm e^{\i kf}}{\i\lambda f}\e^{\i\frac{k}{2f}(x^2+y^2)}\iint\limits_{-\infty}^{+\infty} E_\mathrm{SLM}(x', y')\,\e^{\i\frac{k}{2f}(x'^2 + y'^2)}\e^{-\i\frac{2\pi}{\lambda f}(xx'+yy')}\;\mathrm dx'\mathrm dy'
\end{align}

\begin{align}
E_\mathrm{Lens}^+(x,y) = E_\mathrm{Lens}^-(x,y)\e^{-\i\frac{k}{2f}(x^2+y^2)}
\end{align}

%\begin{align}
%E_\mathrm{Lense}^+(x,y) = \frac{\mathrm e^{\i kf}}{\i\lambda f}\iint\limits_{-\infty}^{+\infty} E_\mathrm{SLM}(x', y')\,\e^{\i\frac{k}{2f}(x'^2 + y'^2)}\e^{-\i\frac{2\pi}{\lambda f}(xx'+yy')}\;\mathrm dx'\mathrm dy'
%\end{align}

Propagate from $E_\mathrm{Lense}^+(x,y)$ to the focal plane:
\begin{align}
E_\mathrm{Focus}(x,y) = \frac{\mathrm e^{\i kf}}{\i\lambda f}\e^{\i\frac{k}{2f}(x^2+y^2)}\iint\limits_{-\infty}^{+\infty} E_\mathrm{Lens}^+(x', y')\,\e^{\i\frac{k}{2f}(x'^2 + y'^2)}\e^{-\i\frac{2\pi}{\lambda f}(xx'+yy')}\;\mathrm dx'\mathrm dy'
\end{align}

...:
\begin{align}
E_\mathrm{Focus}(x,y) &= \frac{\mathrm e^{\i kf}}{\i\lambda f}\e^{\i\frac{k}{2f}(x^2+y^2)}\iint\limits_{-\infty}^{+\infty} E_\mathrm{Lens}^-(x', y')\,\e^{-\i\frac{2\pi}{\lambda f}(xx'+yy')}\;\mathrm dx'\mathrm dy' \\ 
&= \frac{\mathrm e^{\i kf}}{\i\lambda f}\e^{\i\frac{k}{2f}(x^2+y^2)}\,\,4\pi^2\,\check{E}_\mathrm{Lens}^{-}(f_x, f_y)
\end{align}

\begin{align}
\check{E}_\mathrm{Lens}^{-}(f_x, f_y) = \e^{\i kf}\e^{-\i\pi\lambda f(f_x^2+f_y^2)}\,4\pi^2\,\check{E}_\mathrm{SLM}^{-}(f_x, f_y)
\end{align}


$f_x = x/(\lambda f)$, $f_y = y/(\lambda f)$
\begin{align}
\boxed{
E_\mathrm{Focus}(x,y) =  \frac{\mathrm e^{2\i kf}}{\i\lambda f}\,4\pi^2\,\check{E}_\mathrm{SLM}(f_x, f_y)
}
\label{Eq:EFocusXY}
\end{align}

Let's consider a the relation between the field at the SLM plane and the field at the planes different but close to the focal we find:

\begin{align}
E_\mathrm{Focus}(x,y,z) = \frac{\mathrm e^{\i k(f+z)}}{\i\lambda (f+z)}\e^{\i\frac{k}{2(f+z)}(x^2+y^2)}\iint\limits_{-\infty}^{+\infty} E_\mathrm{Lens}^+(x', y')\,\e^{\i\frac{k}{2(f+z)}(x'^2 + y'^2)}\e^{-\i\frac{2\pi}{\lambda (f+z)}(xx'+yy')}\;\mathrm dx'\mathrm dy'
\end{align}

\begin{align}
\lim\limits_{z \rightarrow 0}\;\frac{k}{2(f + z)} \approx \frac{k}{2 f} - \frac{kz}{2f^2} + \dots
\end{align}

\begin{align}
E_\mathrm{Focus}(x,y,z) \approx \frac{\mathrm e^{\i kf}}{\i\lambda f}\e^{\i\frac{k}{2f}(x^2+y^2)}\e^{-\i\frac{kz}{2f^2}(x^2+y^2)}\iint\limits_{-\infty}^{+\infty} E_\mathrm{Lens}^-(x', y')\,\e^{-\i\frac{kz}{2f^2}(x'^2 + y'^2)}\e^{-\i\frac{2\pi}{\lambda f}(xx'+yy')}\;\mathrm dx'\mathrm dy'
\end{align}

\begin{align}
E_\mathrm{Focus}(x,y,z) = \frac{\mathrm e^{\i kf}}{\i\lambda f}\e^{\i\frac{k}{2f}(x^2+y^2)}\e^{-\i\frac{kz}{2f^2}(x^2+y^2)}\mathcal F\left\{E_\mathrm{Lens}^-(x, y)\,\e^{-\i\frac{kz}{2f^2}(x^2 + y^2)}\right\}
\end{align}

\begin{align}
\mathcal F\left\{E_\mathrm{Lens}^-(x, y)\,\e^{-\i\frac{kz}{2f^2}(x^2 + y^2)}\right\} = \e^{\i k(f+z)}\e^{-\i\pi\lambda (f+z)(f_x^2+f_y^2)}\,4\pi^2\,\mathcal F\left\{E_\mathrm{SLM}(x, y)\,\e^{-\i\frac{kz}{2f^2}(x^2 + y^2)}\right\}
\end{align}

\begin{align}
\e^{-\i\pi\lambda (f+z)(f_x^2+f_y^2)} = \e^{-\i\frac{\pi\lambda (f+z)}{\lambda^2f^2}(x^2+y^2)} = \e^{-\i\frac{k}{2f}}\e^{-\i\frac{kz}{2f^2}}
\end{align}


\begin{align}
E_\mathrm{Focus}(x,y,z) \approx \frac{\mathrm e^{\i k(2f + z)}}{\i\lambda f}\e^{\i\frac{k}{2f}(x^2+y^2)}\e^{-\i\frac{kz}{2f^2}(x^2+y^2)}\e^{-\i\frac{k}{2f}(x^2+y^2)}\e^{-\i\frac{kz}{2f^2}(x^2+y^2)}\mathcal F\left\{E_\mathrm{SLM}(x, y)\,\e^{-\i\frac{kz}{2f^2}(x^2 + y^2)}\right\}
\end{align}



\begin{align}
\boxed{
E_\mathrm{Focus}(x,y,z) \approx \frac{\mathrm e^{\i k(2f + z)}}{\i\lambda f}\e^{-\i\frac{kz}{f^2}(x^2+y^2)}\mathcal F\left\{E_\mathrm{SLM}(x, y)\,\e^{-\i\frac{kz}{2f^2}(x^2 + y^2)}\right\}
}
\label{Eq:EFocusXYZ}
\end{align}

In the following, we will consider the incoming beam to be a uniform plane wave, \textit{i.e.}, $E_\mathrm{Beam}(x, y) = E_0$. The SLM is typically a two-dimensional pixellated device whose pixels have area $d^2$, row index $n_x = 1, \dots , N_x$ and column index $n_y = 1, \dots , N_y$. The complex amplitude imposed on the incoming beam by pixel $(n_x , n_y)$ is $\alpha_{n_x, n_y} = \alpha \exp(\i\varphi_{n_x ,n_y})$, where $A$ is an attenuation constant and $\varphi_{n_x ,n_y}$ the phase shift. Therefore, the electric field after the SLM is $E_{n_x, n_y} = E_0\, \alpha\,\exp(\i\varphi_{n_x ,n_y})$. From Eq. (\ref{Eq:EFocusXYZ}) we can now calculate the electric field in the trap volume around the focal plane of the objective as:
\begin{align}
E_\mathrm{Focus}(x,y,z) = \frac{\mathrm e^{\i \frac{2\pi}{\lambda}(2f + z)}}{\i\lambda f}\e^{-\i\frac{2\pi z}{\lambda f^2}(x^2+y^2)}d^2\sum_{n_x=1}^{N_x}\sum_{n_y=1}^{N_y} E_0\,\alpha\,\mathrm e^{\mathrm i \varphi_{n_x ,n_y} -\i\frac{\pi z}{\lambda f^2}(x^2 + y^2) -\i\frac{2\pi}{\lambda f}(x_{n_x,n_y} x + y_{n_x,n_y}y)}
\end{align}
\begin{align}
E_\mathrm{Focus}(x,y,z) = \frac{\mathrm e^{\i \frac{2\pi}{\lambda}(2f + z)}}{\i\lambda f}\e^{-\i\frac{2\pi z}{\lambda f^2}(x^2+y^2)}d^2\sum_{n_x=1}^{N_x}\sum_{n_y=1}^{N_y} E_0\,\alpha\,\mathrm e^{\i\left(\varphi_{n_x ,n_y} - \Delta_{n_x ,n_y}(x, y, z)\right)}
\end{align}
\begin{align}
\Delta_{n_x ,n_y}(x, y ,z) = \frac{2\pi}{\lambda f}(x_{n_x,n_y} x + y_{n_x,n_y}y) + \frac{\pi z}{\lambda f^2}(x^2 + y^2)
\end{align}
The power, \textit{i.e.}, the total, time-averaged energy flux, right after the SLM is ($P_0 = I_0 A_\mathrm{SLM}$):
\begin{align}
P_0 = \frac{c\varepsilon_0}{2}N_xN_y\,d^2\left|E_0\right|^2\alpha^2
\end{align}
The time-averaged energy flux through a diffration-limited spot with area $f^2\lambda^2/(N_xN_yd^2)$ at $(x,y,z)$ is:
\begin{align*}
P(x,y,z) = \frac{c\varepsilon_0}{2}\frac{f^2\lambda^2}{N_xN_yd^2} \left|E_\mathrm{Focus}(x,y,z)\right|^2 = \frac{c\varepsilon_0}{2}\frac{f^2\lambda^2}{N_xN_yd^2}\frac{d^4}{\lambda^2f^2}\left|E_0\right|^2\alpha^2\left|\sum_{n_x=1}^{N_x}\sum_{n_y=1}^{N_y} \mathrm e^{\i\left(\varphi_{n_x ,n_y} - \Delta_{n_x ,n_y}(x, y, z)\right)}\right|^2
\end{align*}
We introduce the dimensionless variable:
\begin{align}
\boxed{
V(x,y,z) = \frac{1}{N_xN_y}\sum_{n_x=1}^{N_x}\sum_{n_y=1}^{N_y} \mathrm e^{\i\left(\varphi_{n_x ,n_y} - \Delta_{n_x ,n_y}(x, y, z)\right)}
}\ ,
\end{align}
defined as: 
\begin{align}
\left|V(x,y,z)\right|^2 = \frac{P(x,y,z)}{P_0}\ .
\end{align}
\end{document}